src/Init/Data/Order/Factories.lean
@@ -147,7 +147,7 @@ public theorem LawfulOrderMin.of_min_le {α : Type u} [Min α] [LE α]
 This lemma characterizes in terms of `LE α` when a `Max α` instance "behaves like a supremum
 operator".
 -/
-public def LawfulOrderSup.of_le {α : Type u} [Max α] [LE α]
+public theorem LawfulOrderSup.of_le {α : Type u} [Max α] [LE α]
     (max_le_iff : ∀ a b c : α, max a b ≤ c ↔ a ≤ c ∧ b ≤ c) : LawfulOrderSup α where
   max_le_iff := max_le_iff
 
@@ -159,7 +159,7 @@ instances.
 
 The produced instance entails `LawfulOrderSup α` and `MaxEqOr α`.
 -/
-public def LawfulOrderMax.of_max_le_iff {α : Type u} [Max α] [LE α]
+public theorem LawfulOrderMax.of_max_le_iff {α : Type u} [Max α] [LE α]
     (max_le_iff : ∀ a b c : α, max a b ≤ c ↔ a ≤ c ∧ b ≤ c := by exact LawfulOrderInf.le_min_iff)
     (max_eq_or : ∀ a b : α, max a b = a ∨ max a b = b := by exact MaxEqOr.max_eq_or) :
     LawfulOrderMax α where
@@ -196,7 +196,7 @@ Creates a *total* `LE α` instance from an `LT α` instance.
 
 This only makes sense for asymmetric `LT α` instances (see `Std.Asymm`).
 -/
-@[inline]
+@[inline, instance_reducible, expose]
 public def _root_.LE.ofLT (α : Type u) [LT α] : LE α where
   le a b := ¬ b < a
 
@@ -275,7 +275,7 @@ public theorem LawfulOrderMin.of_lt {α : Type u} [Min α] [LT α]
 This lemma characterizes in terms of `LT α` when a `Max α` instance
 "behaves like an supremum operator" with respect to `LE.ofLT α`.
 -/
-public def LawfulOrderSup.of_lt {α : Type u} [Max α] [LT α]
+public theorem LawfulOrderSup.of_lt {α : Type u} [Max α] [LT α]
     (lt_max_iff : ∀ a b c : α, c < max a b ↔ c < a ∨ c < b) :
     haveI := LE.ofLT α
     LawfulOrderSup α :=
@@ -291,7 +291,7 @@ Derives a `LawfulOrderMax α` instance for `LE.ofLT` from two properties involvi
 
 The produced instance entails `LawfulOrderSup α` and `MaxEqOr α`.
 -/
-public def LawfulOrderMax.of_lt {α : Type u} [Max α] [LT α]
+public theorem LawfulOrderMax.of_lt {α : Type u} [Max α] [LT α]
     (lt_max_iff : ∀ a b c : α, c < max a b ↔ c < a ∨ c < b)
     (max_eq_or : ∀ a b : α, max a b = a ∨ max a b = b) :
     haveI := LE.ofLT α
