src/Init/Data/Iterators/Consumers/Monadic/Loop.lean
@@ -158,7 +158,7 @@ This is the default implementation of the `IteratorLoop` class.
 It simply iterates through the iterator using `IterM.step`. For certain iterators, more efficient
 implementations are possible and should be used instead.
 -/
-@[always_inline, inline, expose]
+@[always_inline, inline, expose, instance_reducible]
 def IteratorLoop.defaultImplementation {α : Type w} {m : Type w → Type w'} {n : Type x → Type x'}
     [Monad n] [Iterator α m β] :
     IteratorLoop α m n where
@@ -210,7 +210,7 @@ theorem IteratorLoop.wellFounded_of_productive {α β : Type w} {m : Type w → 
 /--
 This `ForIn'`-style loop construct traverses a finite iterator using an `IteratorLoop` instance.
 -/
-@[always_inline, inline]
+@[always_inline, inline, expose, instance_reducible]
 def IteratorLoop.finiteForIn' {m : Type w → Type w'} {n : Type x → Type x'}
     {α : Type w} {β : Type w} [Iterator α m β] [IteratorLoop α m n] [Monad n]
     (lift : ∀ γ δ, (γ → n δ) → m γ → n δ) :
@@ -223,7 +223,7 @@ A `ForIn'` instance for iterators. Its generic membership relation is not easy t
 so this is not marked as `instance`. This way, more convenient instances can be built on top of it
 or future library improvements will make it more comfortable.
 -/
-@[always_inline, inline]
+@[always_inline, inline, expose, instance_reducible]
 def IterM.instForIn' {m : Type w → Type w'} {n : Type w → Type w''}
     {α : Type w} {β : Type w} [Iterator α m β] [IteratorLoop α m n] [Monad n]
     [MonadLiftT m n] :
@@ -238,7 +238,7 @@ instance IterM.instForInOfIteratorLoop {m : Type w → Type w'} {n : Type w → 
   instForInOfForIn'
 
 /-- Internal implementation detail of the iterator library. -/
-@[always_inline, inline]
+@[always_inline, inline, expose, instance_reducible]
 def IterM.Partial.instForIn' {m : Type w → Type w'} {n : Type w → Type w''}
     {α : Type w} {β : Type w} [Iterator α m β] [IteratorLoop α m n] [MonadLiftT m n] [Monad n] :
     ForIn' n (IterM.Partial (α := α) m β) β ⟨fun it out => it.it.IsPlausibleIndirectOutput out⟩ where
@@ -246,7 +246,7 @@ def IterM.Partial.instForIn' {m : Type w → Type w'} {n : Type w → Type w''}
     haveI := @IterM.instForIn'; forIn' it.it init f
 
 /-- Internal implementation detail of the iterator library. -/
-@[always_inline, inline]
+@[always_inline, inline, expose, instance_reducible]
 def IterM.Total.instForIn' {m : Type w → Type w'} {n : Type w → Type w''}
     {α : Type w} {β : Type w} [Iterator α m β] [IteratorLoop α m n] [MonadLiftT m n] [Monad n]
     [Finite α m] :
