src/Init/Data/Range/Polymorphic/RangeIterator.lean
@@ -588,8 +588,7 @@ instance Iterator.instLawfulIteratorLoop [UpwardEnumerable α] [LE α] [Decidabl
     LawfulIteratorLoop (Rxc.Iterator α) Id n where
   lawful := by
     intro lift instLawfulMonadLiftFunction γ it init Pl wf f
-    simp +instances only [IteratorLoop.defaultImplementation, IteratorLoop.forIn,
-      IterM.DefaultConsumers.forIn'_eq_wf Pl wf]
+    simp +instances only [IteratorLoop.forIn, IterM.DefaultConsumers.forIn'_eq_wf Pl wf]
     rw [IterM.DefaultConsumers.forIn'.wf]
     split; rotate_left
     · simp [Monadic.step_eq_step, Monadic.step, Internal.LawfulMonadLiftBindFunction.liftBind_pure]
@@ -1160,8 +1159,7 @@ instance Iterator.instLawfulIteratorLoop [UpwardEnumerable α] [LT α] [Decidabl
     LawfulIteratorLoop (Rxo.Iterator α) Id n where
   lawful := by
     intro lift instLawfulMonadLiftFunction γ it init Pl wf f
-    simp +instances only [IteratorLoop.defaultImplementation, IteratorLoop.forIn,
-      IterM.DefaultConsumers.forIn'_eq_wf Pl wf]
+    simp +instances only [IteratorLoop.forIn, IterM.DefaultConsumers.forIn'_eq_wf Pl wf]
     rw [IterM.DefaultConsumers.forIn'.wf]
     split; rotate_left
     · simp [Monadic.step_eq_step, Monadic.step, Internal.LawfulMonadLiftBindFunction.liftBind_pure]
@@ -1626,8 +1624,7 @@ instance Iterator.instLawfulIteratorLoop [UpwardEnumerable α]
     LawfulIteratorLoop (Rxi.Iterator α) Id n where
   lawful := by
     intro lift instLawfulMonadLiftFunction γ it init Pl wf f
-    simp +instances only [IteratorLoop.defaultImplementation, IteratorLoop.forIn,
-      IterM.DefaultConsumers.forIn'_eq_wf Pl wf]
+    simp +instances only [IteratorLoop.forIn, IterM.DefaultConsumers.forIn'_eq_wf Pl wf]
     rw [IterM.DefaultConsumers.forIn'.wf]
     split; rotate_left
     · simp [Monadic.step_eq_step, Monadic.step, Internal.LawfulMonadLiftBindFunction.liftBind_pure]
